store defined

coq_src/views/rcumeta/Semantics.v
@@ -6,7 +6,148 @@ Require Import Tactics.
 Require Import Setof.
 
 
+  (*Variables*)
+  Definition Var := nat.
+  Proposition Var_eq_dec : forall (x y : Var), {x = y} + {x <> y}.
+   decide equality.
+  Qed.
+  Definition Other := unit.
 
-Module RCUSemantics (ht:HeapTypes)
+  (*Locations*)
+  Definition Loc:= nat.
+  Lemma Loc_eq_dec : forall (x y: Loc), {x=y}+{x <> y}.
+  Proof.
+    decide equality.
+  Qed.
+  
+ (*Values are locations or others*)
+  Inductive Val : Type :=
+  |loc_val : Loc -> Val
+  |oth_val : Other -> Val.
 
-End RCUSemantics.
+  Inductive  FName : Type:=
+  |det : nat -> FName
+  |alt: list nat -> FName
+  .
+
+  Lemma FName_eq_dec: forall (f1 f2: FName),  {f1=f2}+{f1 <> f2}.
+  Proof.
+    induction f1;decide equality.
+    decide equality.
+    decide equality.
+    decide equality.
+    decide equality.
+    decide equality.
+    decide equality.
+  Qed.
+
+  
+  Definition TID:=nat.
+  Inductive Thread : Type:=
+  |reader |writer.
+
+  (*Stores consist of finite partial heap.
+    Finiteness is enforced via a explicit bound.
+    There is also a stack in the store.
+   *)
+  
+  Record store:=
+    {
+      heap : Loc * FName -> option Val;
+      stack : Var * TID -> option Loc;
+      heapBound:nat;
+      heapFree: forall (h:Loc*FName) , heapBound <= (fst h) -> heap h  = None
+    }.
+
+  Instance store_equivalence : Equivalence 
+    (fun s1 s2 => heap s1 == heap s2 /\ stack s1 == stack s2).
+  Admitted.
+
+  (* Stores form a setoid *)
+  Instance store_setoid : Setoid store :=
+   { equiv := fun s1 s2 => heap s1 == heap s2 /\ stack s1 == stack s2 }.
+
+  (* The projections are morphisms *)
+  Instance heap_morphism : Proper (equiv ==> equiv) heap.
+   repeat intro.
+   destruct H.
+   rewr trivial.
+  Qed.
+
+    Instance heap_morphism2 : Proper (equiv ==> eq ==> eq) heap.
+   repeat intro; subst.
+   exact (heap_morphism _ _ H y0).
+  Qed.
+
+  Instance stack_morphism : Proper (equiv ==> equiv) stack.
+   repeat intro.
+   destruct H.
+   rewr trivial.
+  Qed.
+  
+    Instance stack_morphism2 : Proper (equiv ==> eq ==> eq) stack.
+   repeat intro; subst.
+   exact (stack_morphism _ _ H y0).
+  Qed.
+
+  (* Defining overwriting: use the max of the
+     bounds as the new bound.
+   *)
+  Require Import Arith.
+  Import Max. 
+  Lemma max_over_bound (s1 s2 : store) :
+      forall (m:Loc*FName), max (heapBound s1) (heapBound s2) <= (fst m) ->
+          (pw_over (heap s1) (heap s2)) m = None.
+   intros.
+   assert (heap s1 m = None).    
+    apply heapFree; eapply max_lub_l; eauto.
+   unfold pw_over.
+   rewrite H0.
+   apply heapFree; eapply max_lub_r; eauto.
+  Qed.
+
+  Definition overwrite (s1 s2 : store) :=
+   {|
+      heap := pw_over (heap s1) (heap s2);
+      stack := pw_over (stack s1) (stack s2);
+      heapBound := max (heapBound s1) (heapBound s2);
+      heapFree := max_over_bound s1 s2
+   |}.
+
+  (* A store with a single heap cell *)
+  Definition sngloc (h:Loc*FName) (v:Val) : Loc*FName  -> option Val :=
+    fun h' => if Loc_eq_dec  (fst h) (fst h')  then Some v else None.
+
+  (* Bound will be location plus one *)
+  Lemma sngloc_bound (h:Loc*FName) (v:Val) : forall (h':Loc*FName), S (fst h)  <= (fst h') -> sngloc h v h' = None.
+   intros.
+   cbv.
+   destruct (Loc_eq_dec (fst h)  (fst h')).
+   subst.
+   set (Le.le_Sn_n (fst h')).
+(*
+   contradiction.
+   trivial.*)
+Admitted.
+
+  Definition slstore h v : store :=
+    {| heap :=  sngloc h v;
+       stack := fun _ => None;
+       heapBound := S (fst h);
+       heapFree := sngloc_bound h v
+    |}.
+  
+    (* A store with just a single stack variable *) 
+  Definition sngvar (x : Var * TID) (v : Loc) : Var*TID -> option Loc :=
+    fun x' => if Var_eq_dec (fst x) (fst x') then Some v else None.
+
+  Definition svstore x v : store :=
+   {|
+     heap := fun _ => None;
+     stack := sngvar x v;
+     heapBound := 0;
+     heapFree := fun (m : Loc*FName) (_ : 0 <= (fst m)) => eq_refl
+   |}.
+
+
+  
